UnreachableCodeAnalysisCorrect.v
@@ -6,23 +6,6 @@ Require Import Analysis AnalysisForward UnreachableCodeAnalysis UnreachableCode 
 
 Set Implicit Arguments.
 
-Lemma forward_getAnn (sT:stmt) (Dom : stmt -> Type) `{BoundedSemiLattice (Dom sT)}
-      (f: forall sT, list params ->
-                forall s, subTerm s sT -> Dom sT -> anni (Dom sT)) s (ST:subTerm s sT) ZL a an
-  : ann_R eq (fst (@forward sT Dom _ _ f ZL s ST (setTopAnn an a))) an
-    -> getAnn an = a.
-Proof.
-  intros. destruct s, an; inv H1; simpl in *; eauto;
-  repeat let_case_eq; repeat simpl_pair_eqs; subst; simpl in *; inv H2; eauto.
-Qed.
-
-Lemma setTopAnn_eta A (an:ann A) a
-  : getAnn an = a
-    -> setTopAnn an a = an.
-Proof.
-  intros; destruct an; simpl in *; subst; eauto.
-Qed.
-
 Local Arguments proj1_sig {A} {P} e.
 Local Arguments length {A} e.
 Local Arguments forward {sT} {Dom} {H} {H0} ftransform ZL st ST a.
@@ -62,6 +45,78 @@ Proof.
       destruct x0, y0; simpl in *; inv pf; econstructor; eauto.
       destruct b, b0, y0; simpl in *; eauto.
 Qed.
+
+Instance impb_trans : Transitive impb.
+Proof.
+  hnf; intros [] [] []; simpl; intros; eauto.
+Qed.
+
+Lemma PIR2_fold_ojoin_inv A B C
+  : PIR2 (fstNoneOrR impb) (fold_left (zip (ojoin _ join)) A B) C
+    -> (forall n a, get A n a -> length a = length B)
+    -> PIR2 (fstNoneOrR impb) B C.
+Proof.
+  intros.
+  general induction A; simpl in *; eauto.
+  eapply IHA; eauto using get.
+  etransitivity; eauto.
+  exploit PIR2_ojoin_fold as X; [ | | eapply X]; eauto.
+  eapply PIR2_fstNoneOrR_inv_left. reflexivity.
+  erewrite <- H0; eauto using get.
+Qed.
+
+
+Lemma get_union_union_b X `{BoundedSemiLattice X} (A:list (list X)) (b:list X) n x
+  : get b n x
+    -> (forall n a, get A n a -> ❬a❭ = ❬b❭)
+    -> exists y, get (fold_left (zip join) A b) n y /\ poLe x y.
+Proof.
+  intros GETb LEN. general induction A; simpl in *.
+  - eexists x. eauto with cset.
+  - exploit LEN; eauto using get.
+    edestruct (get_length_eq _ GETb (eq_sym H1)) as [y GETa]; eauto.
+    exploit (zip_get join GETb GETa).
+    + exploit IHA; try eapply GET; eauto.
+      rewrite zip_length2; eauto using get with len.
+      edestruct H3; dcr; subst. eexists; split; eauto.
+      rewrite <- H8; eauto. eapply join_poLe.
+Qed.
+
+
+Lemma get_union_union_A X `{BoundedSemiLattice X} (A:list (list X)) a b n k x
+  : get A k a
+    -> get a n x
+    -> (forall n a, get A n a -> ❬a❭ = ❬b❭)
+    -> exists y, get (fold_left (zip join) A b) n y /\ poLe x y.
+Proof.
+  intros GETA GETa LEN.
+  general induction A; simpl in * |- *; isabsurd.
+  inv GETA; eauto.
+  - exploit LEN; eauto using get.
+    edestruct (get_length_eq _ GETa H1) as [y GETb].
+    exploit (zip_get join GETb GETa).
+    exploit (@get_union_union_b _ _ _ A); eauto.
+    rewrite zip_length2; eauto using get with len.
+    destruct H3; dcr; subst. eexists; split; eauto.
+    rewrite <- H5; eauto. rewrite join_commutative.
+    eapply join_poLe.
+  - exploit IHA; eauto.
+    rewrite zip_length2; eauto using get.
+    symmetry; eauto using get.
+Qed.
+
+(*
+Lemma get_olist_union_A' X `{OrderedType X} A a b n k x p
+  : get A k a
+    -> get a n (Some x)
+    -> (forall n a, get A n a -> ❬a❭ = ❬b❭)
+    -> get (olist_union A b) n p
+    -> exists s, p = (Some s) /\ x ⊆ s.
+Proof.
+  intros. edestruct get_olist_union_A; eauto; dcr.
+  get_functional; eauto.
+Qed.
+*)
 
 Definition unreachable_code_analysis_correct sT ZL BL s a (ST:subTerm s sT)
   : ann_R poEq (fst (forward unreachable_code_transform ZL s ST a)) a
@@ -103,12 +158,73 @@ Proof.
   - inv EQ.
     econstructor; eauto.
     + eapply IHAnn; eauto.
+      erewrite (take_eta ❬s❭) at 1. rewrite map_app. eapply PIR2_app; eauto.
+      *
+        eapply PIR2_get. intros. inv_get.
+        destruct x; econstructor.
+        edestruct (get_forwardF (fun _ => bool) (forward unreachable_code_transform)
+                                (fst ⊝ s ++ ZL) (subTerm_EQ_Fun2 eq_refl ST) H12 H4 H3).
+        edestruct (@get_union_union_b (option bool) _ (option_boundedsemilattice _)).
+        eapply H3.
+        Focus 2. dcr.
+        exploit H17. eapply zip_get. eapply map_get_1; eauto.
+        eapply H14. eauto. eapply ann_R_get in H13. rewrite <- H13.
+        inv H15; simpl. rewrite getAnn_setTopAnn. eapply H20.
+        intros.
+        inv_get.
+        edestruct (@forwardF_get _ _ _ _ _ _ _ _ _ _ _ _ H13). dcr.
+        destruct x7; subst;
+        repeat rewrite (@forward_length sT (fun _ => bool)); eauto with len.
+        rewrite Take.take_less_length. eauto with len.
+        repeat rewrite (@forward_length sT (fun _ => bool)); eauto with len.
+      * etransitivity; eauto. eapply PIR2_drop.
+        eapply PIR2_fold_ojoin_inv. reflexivity.
+        intros.
+        inv_get.
+        edestruct (@forwardF_get _ _ _ _ _ _ _ _ _ _ _ _ H3). dcr.
+        destruct x4; subst;
+        repeat rewrite (@forward_length sT (fun _ => bool)); eauto with len.
+    + intros.
+(*            edestruct (get_forwardF (fun _ => bool) (forward unreachable_code_transform)
+                              (fst ⊝ s ++ ZL) (subTerm_EQ_Fun2 eq_refl ST) H3 H4). *)
+      eapply H1 with (ST:=(subTerm_EQ_Fun2 eq_refl ST H3)); eauto.
+      * assert (
+            n < ❬(snd (forward unreachable_code_transform (fst ⊝ s ++ ZL) t (subTerm_EQ_Fun1 eq_refl ST) ta))❭). {
+          repeat rewrite (@forward_length sT (fun _ => bool)). rewrite app_length. rewrite map_length.
+          eapply get_range in H3. omega.
+        }
+        edestruct get_in_range; eauto.
+        edestruct (get_forwardF (fun _ => bool) (forward unreachable_code_transform)
+                                (fst ⊝ s ++ ZL) (subTerm_EQ_Fun2 eq_refl ST) H3 H4 g).
+        assert (n <
+                ❬snd (match x with
+         | ⎣ al' ⎦ =>
+             forward unreachable_code_transform (fst ⊝ s ++ ZL) (snd Zs) x0 (setTopAnn a0 al')
+         | ⎣⎦ => (setAnn (⊥) (snd Zs), tab ⎣⎦ ‖fst ⊝ s ++ ZL‖)
+                      end)❭). {
+          destruct x.
+          erewrite (@forward_length sT (fun _ => bool)). rewrite app_length,map_length.
+          eapply get_range in H3. omega.
+          simpl. rewrite map_length, app_length, map_length.
+          eapply get_range in H3. omega.
+        }
+        edestruct get_in_range; eauto.
+        exploit (@get_union_union_A (option bool) _ (option_boundedsemilattice _)).
+        eapply map_get_1. apply g0. instantiate (3:=snd). eauto.
+        Focus 2.
+        destruct H13; dcr.
+        exploit H17.
+        eapply zip_get.
+        eapply map_get_1. eauto. eapply H15. eauto.
+        destruct x. admit.
+        simpl in *. inv_get. admit.
 
-    + intros.
-      edestruct (get_forwardF (fun _ => bool) (forward unreachable_code_transform)
-                              (fst ⊝ s ++ ZL) (subTerm_EQ_Fun2 eq_refl ST) H3 H4).
-      eapply H1; eauto. admit.
-    + intros.
+        clear_all. intros. inv_get.
+        edestruct (@forwardF_get _ _ _ _ _ _ _ _ _ _ _ _ H). dcr.
+        destruct x4; subst;
+          repeat erewrite (@forward_length sT (fun _ => bool)); eauto with len.
+      * admit.
+    + intros. admit.
 
 Qed.
 
